????

CBPV/ANF.lean
@@ -7,16 +7,16 @@ open Nat ValType ComType Val Com
   A-normal translation continuations
 -----------------------------------*-/
 
-inductive K : Type where
-  | nil : K
-  | app : Val → K → K
-  | letin : Com → K
-  | fst : K → K
-  | snd : K → K
+inductive K : Nat → Type where
+  | nil {δ} : K δ
+  | app {δ} : Val → K δ → K δ
+  | letin {δ} : Com δ → K δ
+  | fst {δ} : K δ → K δ
+  | snd {δ} : K δ → K δ
 
 @[simp]
-def plug (n : Com) : K → Com
-  | .nil => n
+def plug {δ} (n : Com 0) : K δ → Com δ
+  | .nil => weakenJCom δ n
   | .app v k => plug (.app n v) k
   | .letin m => .letin n m
   | .fst k => plug (.fst n) k
@@ -24,7 +24,7 @@ def plug (n : Com) : K → Com
 notation:40 k:41 "[" n:41 "]" => plug n k
 
 @[simp]
-def renameK (ξ : Nat → Nat) : K → K
+def renameK {δ} (ξ : Nat → Nat) : K δ → K δ
   | .nil => .nil
   | .app v k => .app (renameVal ξ v) (renameK ξ k)
   | .letin m => .letin (renameCom (lift ξ) m)
@@ -32,33 +32,34 @@ def renameK (ξ : Nat → Nat) : K → K
   | .snd k => .snd (renameK ξ k)
 
 @[simp]
-def substK (σ : Nat → Val) : K → K
+def substK {δ} (σ : Nat → Val) : K δ → K δ
   | .nil => .nil
   | .app v k => .app (substVal σ v) (substK σ k)
   | .letin m => .letin (substCom (⇑ σ) m)
   | .fst k => .fst (substK σ k)
   | .snd k => .snd (substK σ k)
 
-theorem Evals.plug {k m n} (r : m ⇒⋆ n) : (k[m]) ⇒⋆ (k[n]) := by
+theorem Evals.plug {δ m n} {k : K δ} (r : m ⇒⋆ n) : (k[m]) ⇒⋆ (k[n]) := by
   induction k generalizing m n
-  case nil => exact r
+  case nil => exact Evals.weakenJ r
   case app ih => exact ih (.app r)
   case letin => exact .letin r
   case fst ih => exact ih (.fst r)
   case snd ih => exact ih (.snd r)
 
-theorem substPlug {σ n k} : substCom σ (plug n k) = plug (substCom σ n) (substK σ k) := by
+theorem substPlug {δ σ n} {k : K δ} : substCom σ (plug n k) = plug (substCom σ n) (substK σ k) := by
   induction k generalizing n <;> simp
+  case nil => rw [weakenJSubst]
   case app ih | fst ih | snd ih => simp [ih]
 
-theorem substRenameK {ξ σ k} : substK σ (renameK ξ k) = substK (σ ∘ ξ) k := by
+theorem substRenameK {δ ξ σ} {k : K δ} : substK σ (renameK ξ k) = substK (σ ∘ ξ) k := by
   induction k <;> simp
   case app v _ ih => exact ⟨substRenameVal _ _ v, ih⟩
   case letin m => exact (substRename _ _ _ (upLift _ _ _ (λ _ ↦ rfl))).right m
   case fst ih | snd ih => exact ih
 
 @[simp]
-def renameJK (ξ : Nat → Nat) : K → K
+def renameJK {δ δ'} (ξ : Fin δ → Fin δ') : K δ → K δ'
   | .nil => .nil
   | .app v k => .app v (renameJK ξ k)
   | .letin m => .letin (renameJCom ξ m)
@@ -72,12 +73,12 @@ def renameJK (ξ : Nat → Nat) : K → K
     let x ← k₁[...[kᵢ[□]]] in jump 0 x
 --------------------------------------------------*-/
 
-inductive Jump : Type where
-  | no : Jump
-  | yes : K → Com → Jump
+inductive Jump : Nat → Type where
+  | no {δ} : Jump δ
+  | yes {δ} : K (δ + 1) → Com δ → Jump δ
 
 @[simp]
-def K.jumpify : K → Jump
+def K.jumpify {δ} : K δ → Jump δ
   | .nil => .no
   | .letin m => .yes (.letin (jump 0 (var 0))) m
   | .app v k =>
@@ -93,7 +94,8 @@ def K.jumpify : K → Jump
     | .no => .no
     | .yes k' m => .yes (snd k') m
 
-theorem Jump.rename {ξ k k' m} (e : k.jumpify = yes k' m) : (renameK ξ k).jumpify = yes (renameK ξ k') (renameCom (lift ξ) m) := by
+theorem Jump.rename {ξ δ k k'} {m : Com δ} (e : k.jumpify = yes k' m) :
+  (renameK ξ k).jumpify = yes (renameK ξ k') (renameCom (lift ξ) m) := by
   induction k generalizing k' m
   case nil => cases e
   case letin => simp at *; let ⟨ek, em⟩ := e; subst ek em; simp [lift]
@@ -113,7 +115,7 @@ def Val.joinless : Val → Prop
   | thunk m => m.joinless
 
 @[simp]
-def Com.joinless : Com → Prop
+def Com.joinless {δ} : Com δ → Prop
   | force v | ret v => v.joinless
   | lam m | fst m | snd m => m.joinless
   | app n v => n.joinless ∧ v.joinless
@@ -125,8 +127,8 @@ end
 section
 set_option hygiene false
 local notation:1023 "⟦" v "⟧ᵥ" => Aval v
-local notation:1023 "⟦" m "⟧ₘ" => Acom .nil m
-local notation:1022 "⟦" m "⟧ₘ" k => Acom k m
+local notation:1023 "⟦" m "⟧ₘ" => Acom .nil (zero_le 0) m
+local notation:1022 "⟦" m "⟧ₘ" k "#" le => Acom k le m
 mutual
 @[simp]
 def Aval : Val → Val
@@ -137,26 +139,29 @@ def Aval : Val → Val
   | thunk m => .thunk ⟦ m ⟧ₘ
 
 @[simp]
-def Acom (k : K) : Com → Com
+def Acom {δ δ'} (k : K δ) (le : δ' ≤ δ) : Com δ' → Com δ
   | force v => k [ .force ⟦ v ⟧ᵥ ]
   | ret v   => k [ .ret ⟦ v ⟧ᵥ ]
   | lam m   => k [ .lam ⟦ m ⟧ₘ ]
-  | app n v   => ⟦ n ⟧ₘ .app ⟦ v ⟧ᵥ k
-  | letin n m => ⟦ n ⟧ₘ .letin (⟦ m ⟧ₘ renameK succ k)
+  | app n v   => ⟦ n ⟧ₘ .app ⟦ v ⟧ᵥ k # zero_le δ
+  | letin n m => ⟦ n ⟧ₘ .letin (⟦ m ⟧ₘ renameK succ k # le) # zero_le δ
   | prod m₁ m₂ => k [ .prod ⟦ m₁ ⟧ₘ ⟦ m₂ ⟧ₘ ]
-  | fst n => ⟦ n ⟧ₘ .fst k
-  | snd n => ⟦ n ⟧ₘ .snd k
-  | join n m => join (⟦ n ⟧ₘ renameK succ k) (⟦ m ⟧ₘ renameJK succ k)
-  | jump j v => jump j (⟦ v ⟧ᵥ)
+  | fst n => ⟦ n ⟧ₘ .fst k # zero_le δ
+  | snd n => ⟦ n ⟧ₘ .snd k # zero_le δ
+  | join n m => join (⟦ n ⟧ₘ renameK succ k # le)
+                     (⟦ m ⟧ₘ renameJK Fin.succ k # succ_le_succ le)
+  | jump j v => jump (Fin.castLE le j) (⟦ v ⟧ᵥ)
   | case v m₁ m₂ =>
     match k.jumpify with
-    | .no => .case ⟦ v ⟧ᵥ (⟦ m₁ ⟧ₘ renameK succ k) (⟦ m₂ ⟧ₘ renameK succ k)
-    | .yes k m => .join m (.case ⟦ v ⟧ᵥ (⟦ m₁ ⟧ₘ renameK succ k) (⟦ m₂ ⟧ₘ renameK succ k))
+    | .no => .case ⟦ v ⟧ᵥ (⟦ m₁ ⟧ₘ renameK succ k # le) (⟦ m₂ ⟧ₘ renameK succ k # le)
+    | .yes k m =>
+      .join m (.case ⟦ v ⟧ᵥ (⟦ m₁ ⟧ₘ renameK succ k # .step le)
+                            (⟦ m₂ ⟧ₘ renameK succ k # .step le))
 end
 end
 notation:1023 "⟦" v "⟧ᵥ" => Aval v
-notation:1023 "⟦" m "⟧ₘ" => Acom K.nil m
-notation:1022 "⟦" m "⟧ₘ" k => Acom k m
+notation:1023 "⟦" m "⟧ₘ" => Acom K.nil (zero_le 0) m
+notation:1022 "⟦" m "⟧ₘ" k "#" le => Acom k le m
 
 /-*-----------------------------------------------------------------
   Validity of A-normal translation,
@@ -175,7 +180,7 @@ def isVal : Val → Prop
   | _ => True
 
 @[simp]
-def isCom : Com → Prop
+def isCom {δ} : Com δ → Prop
   | force v | ret v => isVal v
   | lam m => isCfg m
   | app n v => isCom n ∧ isVal v
@@ -184,7 +189,7 @@ def isCom : Com → Prop
   | _ => False
 
 @[simp]
-def isCfg : Com → Prop
+def isCfg {δ} : Com δ → Prop
   | letin n m => isCom n ∧ isCfg m
   | case _ m₁ m₂ => isCfg m₁ ∧ isCfg m₂
   | join n m => isCfg n ∧ isCfg m
@@ -193,27 +198,32 @@ def isCfg : Com → Prop
 end
 
 @[simp]
-def isK : K → Prop
+def isK {δ} : K δ → Prop
   | .nil => True
   | .app v k => isVal v ∧ isK k
   | .letin m => isCfg m
   | .fst k | .snd k => isK k
 
-theorem isCom.isCfg {n} (isc : isCom n) : isCfg n := by
+theorem isCom.weakenJ {δ δ'} {n : Com δ} (isc : isCom n) : isCom (weakenJCom δ' n) := by
+  mutual_induction n generalizing isc
+  all_goals simp at * <;> assumption
+
+theorem isCom.isCfg {δ} {n : Com δ} (isc : isCom n) : isCfg n := by
   mutual_induction n generalizing isc
   case letin | case => unfold isCom at isc; contradiction
   all_goals simp [isc] at *
 
-theorem isK.plug {n k} (isk : isK k) (isc : isCom n) : isCfg (k [ n ]) := by
+theorem isK.plug {δ n} {k : K δ} (isk : isK k) (isc : isCom n) : isCfg (k [ n ]) := by
   induction k generalizing n <;> simp at *
-  case nil => exact isc.isCfg
+  case nil => exact isc.weakenJ.isCfg
   case letin => simp [isk, isc]
   case app ih | fst ih | snd ih => apply ih <;> simp [isk, isc]
 
 theorem isRenameValCfg {ξ} :
   (∀ v, isVal v → isVal (renameVal ξ v)) ∧
-  (∀ m, (isCom m → isCom (renameCom ξ m)) ∧
-        (isCfg m → isCfg (renameCom ξ m))) := by
+  (∀ {δ} (m : Com δ),
+    (isCom m → isCom (renameCom ξ m)) ∧
+    (isCfg m → isCfg (renameCom ξ m))) := by
   refine ⟨λ v isv ↦ ?val, λ m ↦ ?com⟩
   mutual_induction v, m generalizing ξ
   all_goals simp at *
@@ -248,31 +258,31 @@ theorem isRenameValCfg {ξ} :
   case jump ih => exact ih
 
 def isVal.rename {ξ v} : isVal v → isVal (renameVal ξ v) := isRenameValCfg.left v
-def isCom.rename {ξ m} : isCom m → isCom (renameCom ξ m) := (isRenameValCfg.right m).left
-def isCfg.rename {ξ m} : isCfg m → isCfg (renameCom ξ m) := (isRenameValCfg.right m).right
+def isCom.rename {ξ δ} {m : Com δ} : isCom m → isCom (renameCom ξ m) := (isRenameValCfg.right m).left
+def isCfg.rename {ξ δ} {m : Com δ} : isCfg m → isCfg (renameCom ξ m) := (isRenameValCfg.right m).right
 
-theorem isCfg.renameJ {ξ} : ∀ m, isCfg m → isCfg (renameJCom ξ m) := by
-  intro m ism; mutual_induction m generalizing ξ ism
+theorem isCfg.renameJ {δ δ'} {ξ : Fin δ → Fin δ'} : ∀ m, isCfg m → isCfg (renameJCom ξ m) := by
+  intro m ism; mutual_induction m generalizing δ' ism
   all_goals simp at *; try assumption
   case letin ih => let ⟨ism, isn⟩ := ism; exact ⟨ism, ih isn⟩
   case case ihm₁ ihm₂ => let ⟨ism₁, ism₂⟩ := ism; exact ⟨ihm₁ ism₁, ihm₂ ism₂⟩
   case join ihn ihm => let ⟨isn, ism⟩ := ism; exact ⟨ihn isn, ihm ism⟩
 
-theorem isK.rename {ξ k} (isk : isK k) : isK (renameK ξ k) := by
+theorem isK.rename {ξ δ} {k : K δ} (isk : isK k) : isK (renameK ξ k) := by
   induction k generalizing ξ
   all_goals simp at *
   case app ih => let ⟨isv, isk⟩ := isk; exact ⟨isv.rename, ih isk⟩
   case letin => exact isk.rename
   case fst ih | snd ih => exact ih isk
 
-theorem isK.renameJ {ξ k} (isk : isK k) : isK (renameJK ξ k) := by
+theorem isK.renameJ {δ δ' k} {ξ : Fin δ → Fin δ'} (isk : isK k) : isK (renameJK ξ k) := by
   induction k generalizing ξ
   all_goals simp at *
   case app ih => let ⟨isv, isk⟩ := isk; exact ⟨isv, ih isk⟩
   case letin => exact isk.renameJ
   case fst ih | snd ih => exact ih isk
 
-theorem isK.jumpify {k k' m} (isk : isK k) (e : k.jumpify = .yes k' m) : isK k' ∧ isCfg m := by
+theorem isK.jumpify {δ k k'} {m : Com δ} (isk : isK k) (e : k.jumpify = .yes k' m) : isK k' ∧ isCfg m := by
   induction k generalizing k' m
   case nil => simp at e
   case letin =>
@@ -292,11 +302,12 @@ theorem isK.jumpify {k k' m} (isk : isK k) (e : k.jumpify = .yes k' m) : isK k' 
       let ⟨isk, ism⟩ := ih isk e'
       exact ⟨isk, ism⟩
 
-theorem isANF : (∀ v, isVal ⟦v⟧ᵥ) ∧ (∀ m k, isK k → isCfg (⟦m⟧ₘ k)) := by
-  refine ⟨λ v ↦ ?val, λ m k ↦ ?com⟩
+theorem isANF : (∀ v, isVal ⟦v⟧ᵥ) ∧
+  (∀ {δ δ'} (m : Com δ') (k : K δ) (le : δ' ≤ δ), isK k → isCfg (⟦m⟧ₘ k # le)) := by
+  refine ⟨λ v ↦ ?val, λ {δ δ'} m k le ↦ ?com⟩
   mutual_induction v, m
   all_goals simp
-  case thunk ih => exact ih _ ⟨⟩
+  case thunk ih => exact ih .nil .refl ⟨⟩
   all_goals intro isk
   case force isv => apply isk.plug; simp [isv]
   case lam ih | ret ih => apply isk.plug; simp [ih]
@@ -304,17 +315,17 @@ theorem isANF : (∀ v, isVal ⟦v⟧ᵥ) ∧ (∀ m k, isK k → isCfg (⟦m⟧
   case letin isc₁ isc₂ => apply isc₁; apply isc₂; simp [isk.rename]
   case prod isc₁ isc₂ => apply isk.plug; simp [isc₁, isc₂]
   case fst isc | snd isc => apply isc; simp [isk]
-  case join isc₁ isc₂ => exact ⟨isc₁ _ (isk.rename), isc₂ _ isk.renameJ⟩
+  case join isc₁ isc₂ => exact ⟨isc₁ _ le (isk.rename), isc₂ _ (succ_le_succ le) isk.renameJ⟩
   case jump ih => exact ih
   case case isc₁ isc₂ =>
     split <;> simp
-    case _ => exact ⟨isc₁ _ (isk.rename), isc₂ _ (isk.rename)⟩
+    case _ => exact ⟨isc₁ _ le (isk.rename), isc₂ _ le (isk.rename)⟩
     case _ e =>
       let ⟨isk, ism⟩ := isk.jumpify e
-      exact ⟨ism, isc₁ _ (isk.rename), isc₂ _ (isk.rename)⟩
+      exact ⟨ism, isc₁ _ (.step le) (isk.rename), isc₂ _ (.step le) (isk.rename)⟩
 
 def Val.ANF : ∀ v, isVal ⟦v⟧ᵥ := isANF.left
-def Com.ANF : ∀ m, isCfg ⟦m⟧ₘ := λ m ↦ isANF.right m .nil ⟨⟩
+def Com.ANF : ∀ m, isCfg ⟦m⟧ₘ := λ m ↦ isANF.right m .nil .refl ⟨⟩
 
 /-*------------------------------------------
   Type preservation of A-normal translation
@@ -325,53 +336,63 @@ section
 set_option hygiene false
 open K
 local notation:40 Γ:41 "∣" Δ:41 "⊢" k:41 "∶" B₁:41 "⇒" B₂:41 => wtK Γ Δ k B₁ B₂
-inductive wtK : Ctxt → Dtxt → K → ComType → ComType → Prop where
-  | nil {Γ B} :
-    ---------------
-    Γ ∣ ⬝ ⊢ nil ∶ B ⇒ B
-  | app {Γ Δ k v B₁ B₂} {A : ValType} :
+inductive wtK : ∀ {δ}, Ctxt → Dtxt δ → K δ → ComType → ComType → Prop where
+  | nil {Γ δ B} {Δ : Dtxt δ} :
+    -------------------
+    Γ ∣ Δ ⊢ nil ∶ B ⇒ B
+  | app {Γ δ Δ v B₁ B₂} {A : ValType} {k : K δ} :
     Γ ⊢ v ∶ A →
     Γ ∣ Δ ⊢ k ∶ B₁ ⇒ B₂ →
-    -----------------------------
+    ---------------------------------
     Γ ∣ Δ ⊢ app v k ∶ (Arr A B₁) ⇒ B₂
-  | letin {Γ Δ m A} {B : ComType} :
+  | letin {Γ δ Δ A B} {m : Com δ} :
     Γ ∷ A ∣ Δ ⊢ m ∶ B →
-    ---------------------
+    -------------------------
     Γ ∣ Δ ⊢ letin m ∶ F A ⇒ B
-  | fst {Γ Δ k B₁ B₂ B₃} :
+  | fst {Γ δ Δ B₁ B₂ B₃} {k : K δ} :
     Γ ∣ Δ ⊢ k ∶ B₁ ⇒ B₃ →
-    -----------------------------
+    ---------------------------------
     Γ ∣ Δ ⊢ fst k ∶ (Prod B₁ B₂) ⇒ B₃
-  | snd {Γ Δ k B₁ B₂ B₃} :
+  | snd {Γ δ Δ B₁ B₂ B₃} {k : K δ} :
     Γ ∣ Δ ⊢ k ∶ B₂ ⇒ B₃ →
-    -----------------------------
+    ---------------------------------
     Γ ∣ Δ ⊢ snd k ∶ (Prod B₁ B₂) ⇒ B₃
 end
 notation:40 Γ:41 "∣" Δ:41 "⊢" k:41 "∶" B₁:41 "⇒" B₂:41 => wtK Γ Δ k B₁ B₂
 
-theorem wtK.rename {ξ k B₁ B₂} {Γ Ξ : Ctxt} {Δ} (hξ : Ξ ⊢ ξ ∶ Γ) (h : Γ ∣ Δ ⊢ k ∶ B₁ ⇒ B₂) :
+namespace wtK
+
+theorem rename {ξ δ k B₁ B₂} {Γ Ξ : Ctxt} {Δ : Dtxt δ} (hξ : Ξ ⊢ ξ ∶ Γ) (h : Γ ∣ Δ ⊢ k ∶ B₁ ⇒ B₂) :
   Ξ ∣ Δ ⊢ renameK ξ k ∶ B₁ ⇒ B₂ := by
   induction h generalizing ξ Ξ
   all_goals constructor <;> apply_rules [wtRenameVal, wtRenameCom, wRenameLift]
 
-theorem wtK.weaken {Γ Δ k A B₁ B₂} : Γ ∣ Δ ⊢ k ∶ B₁ ⇒ B₂ → Γ ∷ A ∣ Δ ⊢ renameK succ k ∶ B₁ ⇒ B₂ :=
-  wtK.rename wRenameSucc
+theorem weaken {Γ δ Δ A B₁ B₂} {k : K δ} : Γ ∣ Δ ⊢ k ∶ B₁ ⇒ B₂ → Γ ∷ A ∣ Δ ⊢ renameK succ k ∶ B₁ ⇒ B₂ :=
+  rename wRenameSucc
 
-theorem wtK.plug {Γ Δ n k B₁ B₂}
+theorem renameJ {Γ} {δ δ' ξ} {Δ : Dtxt δ} {Φ : Dtxt δ'} {k B₁ B₂} (hξ : Φ ⊢ ξ ∶ Δ) (h : Γ ∣ Δ ⊢ k ∶ B₁ ⇒ B₂) :
+  Γ ∣ Φ ⊢ renameJK ξ k ∶ B₁ ⇒ B₂ := by
+  induction h generalizing δ' Φ
+  all_goals constructor <;> apply_rules [wtRenameJ]
+
+theorem weakenJ {Γ δ Δ A B B₁ B₂} {k : K δ} : Γ ∣ Δ ⊢ k ∶ B₁ ⇒ B₂ → Γ ∣ Δ ∷ A ↗ B ⊢ renameJK .succ k ∶ B₁ ⇒ B₂ :=
+  renameJ wRenameJSucc
+
+theorem plug {Γ δ Δ n B₁ B₂} {k : K δ}
   (hk : Γ ∣ Δ ⊢ k ∶ B₁ ⇒ B₂) (h : Γ ∣ ⬝ ⊢ n ∶ B₁) : Γ ∣ Δ ⊢ (k [ n ]) ∶ B₂ := by
   induction hk generalizing n
-  case nil => exact h
+  case nil => exact wtRenameJ (λ _ _ _ mem ↦ by cases mem) h
   case app hv _ hn => simp; exact hn (.app h hv)
   case letin hm => exact .letin h hm
   case fst hn => exact hn (.fst h)
   case snd hn => exact hn (.snd h)
 
-theorem wtK.jumpify {Γ Δ k k' m B₁ B₂}
+theorem jumpify {Γ δ Δ k' m B₁ B₂} {k : K δ}
   (hk : Γ ∣ Δ ⊢ k ∶ B₁ ⇒ B₂) (e : k.jumpify = .yes k' m) :
   ∃ A, Γ ∣ Δ ∷ A ↗ B₂ ⊢ k' ∶ B₁ ⇒ B₂ ∧ Γ ∷ A ∣ Δ ⊢ m ∶ B₂ := by
-  induction hk generalizing k' m
+  induction hk
   case nil => cases e
-  case letin A _ hm =>
+  case letin A _ _ hm =>
     simp at e; let ⟨ek, em⟩ := e; subst ek em
     exact ⟨A, .letin (.jump .here (.var .here)) , hm⟩
   case app hv _ ih | fst ih | snd ih =>
@@ -382,34 +403,35 @@ theorem wtK.jumpify {Γ Δ k k' m B₁ B₂}
       refine ⟨A, ?_, hm⟩
       all_goals constructor <;> assumption
 
+end wtK
+
 theorem preservation {Γ} :
   (∀ {v} {A : ValType}, v.joinless → Γ ⊢ v ∶ A → Γ ⊢ ⟦ v ⟧ᵥ ∶ A) ∧
-  (∀ {Δ k m} {B₁ B₂ : ComType}, m.joinless → Γ ∣ Δ ⊢ k ∶ B₁ ⇒ B₂ → Γ ∣ ⬝ ⊢ m ∶ B₁ → Γ ∣ Δ ⊢ ⟦ m ⟧ₘ k ∶ B₂) := by
-  refine ⟨λ vj h ↦ ?val, λ mj hk h ↦ ?com⟩
-  case' com => generalize e : Dtxt.nil = Δ' at h
+  (∀ {δ δ'} {Δ : Dtxt δ} {Δ' : Dtxt δ'} {k m} {B₁ B₂ : ComType} le, m.joinless → Γ ∣ Δ ⊢ k ∶ B₁ ⇒ B₂ → Γ ∣ Δ' ⊢ m ∶ B₁ → Γ ∣ Δ ⊢ ⟦ m ⟧ₘ k # le ∶ B₂) := by
+  refine ⟨λ {v A} vj h ↦ ?val, λ {δ δ' Δ Δ' k m B₁ B₂} le mj hk h ↦ ?com⟩
   mutual_induction h, h
   case var mem => exact .var mem
   case unit => exact .unit
   case inl h => exact .inl (h vj)
   case inr h => exact .inr (h vj)
-  case thunk h => exact .thunk (h vj .nil rfl)
-  all_goals subst e
-  case force h _ _ _ => exact (wtK.plug hk (.force (h mj)))
-  case ret h _ _ _ => exact (wtK.plug hk (.ret (h mj)))
-  case lam h _ _ _ => exact (wtK.plug hk (.lam (h mj .nil rfl)))
-  case app hn hv k _ _ => let ⟨nj, vj⟩ := mj; exact hn nj (.app (hv vj) hk) rfl
-  case letin hn _ _ _ _ hm => let ⟨nj, mj⟩ := mj; exact hn nj (.letin (hm mj (wtK.weaken hk) rfl)) rfl
-  case prod hm₁ hm₂ _ _ _ => let ⟨mj₁, mj₂⟩ := mj; exact wtK.plug hk (.prod (hm₁ mj₁ .nil rfl) (hm₂ mj₂ .nil rfl))
-  case fst h _ _ _ => exact h mj (.fst hk) rfl
-  case snd h _ _ _ => exact h mj (.snd hk) rfl
-  case join | jump => simp at mj
-  case case hv _ _ _ _ _ hm₁ hm₂ =>
+  case thunk h => exact .thunk (h .refl vj .nil)
+  case force h => exact (wtK.plug hk (.force (h mj)))
+  case ret h => exact (wtK.plug hk (.ret (h mj)))
+  case lam h => exact (wtK.plug hk (.lam (h .refl mj .nil)))
+  case app hn hv => let ⟨nj, vj⟩ := mj; exact hn (zero_le δ) nj (.app (hv vj) hk)
+  case letin hn hm => let ⟨nj, mj⟩ := mj; exact hn (zero_le δ) nj (.letin (hm le mj (wtK.weaken hk)))
+  case prod hm₁ hm₂ => let ⟨mj₁, mj₂⟩ := mj; exact wtK.plug hk (.prod (hm₁ .refl mj₁ .nil) (hm₂ .refl mj₂ .nil))
+  case fst h => exact h (zero_le δ) mj (.fst hk)
+  case snd h => exact h (zero_le δ) mj (.snd hk)
+  case join hn hm | jump mem _ hv => cases mj
+  -- let ⟨nj, mj⟩ := mj; exact .join (hn le nj (wtK.weaken hk)) (hm (succ_le_succ le) mj (wtK.weakenJ hk))
+  case case hv hm₁ hm₂ =>
     let ⟨vj, mj₁, mj₂⟩ := mj; simp; split
     case _ =>
-      exact .case (hv vj) (hm₁ mj₁ (wtK.weaken hk) rfl) (hm₂ mj₂ (wtK.weaken hk) rfl)
+      exact .case (hv vj) (hm₁ le mj₁ (wtK.weaken hk)) (hm₂ le mj₂ (wtK.weaken hk))
     case _ e =>
       let ⟨_, hk, hm⟩ := hk.jumpify e
-      exact (.join hm (.case (hv vj) (hm₁ mj₁ (wtK.weaken hk) rfl) (hm₂ mj₂ (wtK.weaken hk) rfl)))
+      exact (.join hm (.case (hv vj) (hm₁ (.step le) mj₁ (wtK.weaken hk)) (hm₂ (.step le) mj₂ (wtK.weaken hk))))
 
 def ValWt.preservation {Γ} := @(@_root_.preservation Γ).left
 def ComWt.preservation {Γ} := @(@_root_.preservation Γ).right
@@ -419,7 +441,7 @@ def ComWt.preservation {Γ} := @(@_root_.preservation Γ).right
 --------------------------------------*-/
 
 @[simp]
-def semK (Γ : Ctxt) (Δ : Dtxt) k₁ k₂ B₁ B₂ :=
+def semK (Γ : Ctxt) {δ} (Δ : Dtxt δ) k₁ k₂ B₁ B₂ :=
   ∀ {σ τ}, Γ ⊨ σ ~ τ →
   ∀ {js₁ js₂}, Δ ⊨ js₁ ~ js₂ →
   ∀ {n₁ n₂}, (n₁, n₂) ∈ ⟦B₁⟧ᵉ →
@@ -428,7 +450,7 @@ notation:40 Γ:41 "∣" Δ:41 "⊨" k₁:41 "~" k₂:41 "∶" B₁:41 "⇒" B₂
 
 namespace semK
 
-theorem weaken {Γ Δ k₁ k₂ A B₁ B₂} (h : Γ ∣ Δ ⊨ k₁ ~ k₂ ∶ B₁ ⇒ B₂) : Γ ∷ A ∣ Δ ⊨ renameK succ k₁ ~ renameK succ k₂ ∶ B₁ ⇒ B₂ := by
+theorem weaken {Γ δ} {Δ : Dtxt δ} {k₁ k₂ A B₁ B₂} (h : Γ ∣ Δ ⊨ k₁ ~ k₂ ∶ B₁ ⇒ B₂) : Γ ∷ A ∣ Δ ⊨ renameK succ k₁ ~ renameK succ k₂ ∶ B₁ ⇒ B₂ := by
   intro σ τ hστ js₁ js₂ hjs n₁ n₂ hn
   rw [substRenameK, substRenameK]
   exact h (semCtxt.rename wRenameSucc hστ) hjs hn
@@ -437,34 +459,34 @@ theorem weaken {Γ Δ k₁ k₂ A B₁ B₂} (h : Γ ∣ Δ ⊨ k₁ ~ k₂ ∶ 
   Fundamental theorem for semantic equivalence of continuations
 --------------------------------------------------------------*-/
 
-def nil {Γ Δ B} : Γ ∣ Δ ⊨ .nil ~ .nil ∶ B ⇒ B :=
+def nil {Γ δ B} {Δ : Dtxt δ} : Γ ∣ Δ ⊨ .nil ~ .nil ∶ B ⇒ B :=
   λ _ _ _ _ ↦ ℰ.bwdsRejoin .refl .refl
 
-def fst {Γ Δ k₁ k₂ B₁ B₂ B₃} (h : Γ ∣ Δ ⊨ k₁ ~ k₂ ∶ B₁ ⇒ B₃) : Γ ∣ Δ ⊨ .fst k₁ ~ .fst k₂ ∶ Prod B₁ B₂ ⇒ B₃ := by
+def fst {Γ δ} {Δ : Dtxt δ} {k₁ k₂ B₁ B₂ B₃} (h : Γ ∣ Δ ⊨ k₁ ~ k₂ ∶ B₁ ⇒ B₃) : Γ ∣ Δ ⊨ .fst k₁ ~ .fst k₂ ∶ Prod B₁ B₂ ⇒ B₃ := by
   intro σ τ hστ js₁ js₂ hjs n₁ n₂ hn; simp
   have ⟨n₁₁, n₁₂, n₂₁, n₂₂, rn₁, rn₂, hn₁⟩ := hn.fst
-  refine ℰ.bwds ?_ ?_ (h hστ hjs hn₁)
+  refine ℰ.bwds ?left ?right (h hστ hjs hn₁)
   all_goals refine .rejoin (.plug ?_)
-  . exact .trans' (Evals.fst rn₁) (.once .π1)
-  . exact .trans' (Evals.fst rn₂) (.once .π1)
+  case left  => rw [← @weakenJCom0 n₁₁]; exact .trans' (Evals.fst rn₁) (.once .π1)
+  case right => rw [← @weakenJCom0 n₂₁]; exact .trans' (Evals.fst rn₂) (.once .π1)
 
-def snd {Γ Δ k₁ k₂ B₁ B₂ B₃} (h : Γ ∣ Δ ⊨ k₁ ~ k₂ ∶ B₂ ⇒ B₃) : Γ ∣ Δ ⊨ .snd k₁ ~ .snd k₂ ∶ Prod B₁ B₂ ⇒ B₃ := by
+def snd {Γ δ} {Δ : Dtxt δ} {k₁ k₂ B₁ B₂ B₃} (h : Γ ∣ Δ ⊨ k₁ ~ k₂ ∶ B₂ ⇒ B₃) : Γ ∣ Δ ⊨ .snd k₁ ~ .snd k₂ ∶ Prod B₁ B₂ ⇒ B₃ := by
   intro σ τ hστ js₁ js₂ hjs n₁ n₂ hn; simp
   have ⟨n₁₁, n₁₂, n₂₁, n₂₂, rn₁, rn₂, hn₂⟩ := hn.snd
-  refine ℰ.bwds ?_ ?_ (h hστ hjs hn₂)
+  refine ℰ.bwds ?left ?right (h hστ hjs hn₂)
   all_goals refine .rejoin (.plug ?_)
-  . exact .trans' (Evals.snd rn₁) (.once .π2)
-  . exact .trans' (Evals.snd rn₂) (.once .π2)
+  case left  => rw [← @weakenJCom0 n₁₂]; exact .trans' (Evals.snd rn₁) (.once .π2)
+  case right => rw [← @weakenJCom0 n₂₂]; exact .trans' (Evals.snd rn₂) (.once .π2)
 
-theorem app {Γ Δ v w k₁ k₂ B₁ B₂} {A : ValType} (hA : Γ ⊨ v ~ w ∶ A) (h : Γ ∣ Δ ⊨ k₁ ~ k₂ ∶ B₁ ⇒ B₂) : Γ ∣ Δ ⊨ .app v k₁ ~ .app w k₂ ∶ Arr A B₁ ⇒ B₂ := by
+theorem app {Γ δ} {Δ : Dtxt δ} {v w k₁ k₂ B₁ B₂} {A : ValType} (hA : Γ ⊨ v ~ w ∶ A) (h : Γ ∣ Δ ⊨ k₁ ~ k₂ ∶ B₁ ⇒ B₂) : Γ ∣ Δ ⊨ .app v k₁ ~ .app w k₂ ∶ Arr A B₁ ⇒ B₂ := by
   intro σ τ hστ js₁ js₂ hjs n₁ n₂ hn; simp
   have ⟨_, _, rn₁, rn₂, hm⟩ := hn.lam_inv
-  refine ℰ.bwds ?_ ?_ (h hστ hjs (hm _ _ (hA hστ)))
+  refine ℰ.bwds ?left ?right (h hστ hjs (hm _ _ (hA hστ)))
   all_goals refine .rejoin (.plug ?_)
-  . exact .trans' (Evals.app rn₁) (.once .β)
-  . exact .trans' (Evals.app rn₂) (.once .β)
+  case left w _ => rw [← @weakenJCom0 (w⦃v⦃σ⦄⦄)]; exact .trans' (Evals.app rn₁) (.once .β)
+  case right v  => rw [← @weakenJCom0 (v⦃w⦃τ⦄⦄)]; exact .trans' (Evals.app rn₂) (.once .β)
 
-theorem letin {Γ Δ m₁ m₂ A} {B : ComType} (h : Γ ∷ A ∣ Δ ⊨ m₁ ~ m₂ ∶ B) : Γ ∣ Δ ⊨ .letin m₁ ~ .letin m₂ ∶ F A ⇒ B := by
+theorem letin {Γ δ} {Δ : Dtxt δ} {m₁ m₂ A} {B : ComType} (h : Γ ∷ A ∣ Δ ⊨ m₁ ~ m₂ ∶ B) : Γ ∣ Δ ⊨ .letin m₁ ~ .letin m₂ ∶ F A ⇒ B := by
   intro σ τ hστ js₁ js₂ hjs n₁ n₂ hn
   have ⟨v, w, rn₁, rn₂, hA⟩ := hn.ret_inv
   refine ℰ.bwds ?_ ?_ (h (semCtxt.cons hA hστ) hjs)
@@ -474,7 +496,7 @@ theorem letin {Γ Δ m₁ m₂ A} {B : ComType} (h : Γ ∷ A ∣ Δ ⊨ m₁ ~ 
 
 end semK
 
-theorem soundK {Γ Δ k B₁ B₂} (h : Γ ∣ Δ ⊢ k ∶ B₁ ⇒ B₂) : Γ ∣ Δ ⊨ k ~ k ∶ B₁ ⇒ B₂ := by
+theorem soundK {Γ δ} {Δ : Dtxt δ} {k B₁ B₂} (h : Γ ∣ Δ ⊢ k ∶ B₁ ⇒ B₂) : Γ ∣ Δ ⊨ k ~ k ∶ B₁ ⇒ B₂ := by
   induction h
   case nil => exact semK.nil
   case app hv _ ih => exact semK.app (soundVal hv) ih
@@ -486,30 +508,30 @@ theorem soundK {Γ Δ k B₁ B₂} (h : Γ ∣ Δ ⊢ k ∶ B₁ ⇒ B₂) : Γ 
   Semantic equivalence of plugged continuations
 ----------------------------------------------*-/
 
-theorem semK.plug {Γ Δ n₁ n₂ k₁ k₂ B₁ B₂} (hk : Γ ∣ Δ ⊨ k₁ ~ k₂ ∶ B₁ ⇒ B₂) (hn : Γ ∣ ⬝ ⊨ n₁ ~ n₂ ∶ B₁) : Γ ∣ Δ ⊨ (k₁[n₁]) ~ (k₂[n₂]) ∶ B₂ := by
+theorem semK.plug {Γ δ} {Δ : Dtxt δ} {n₁ n₂ k₁ k₂ B₁ B₂} (hk : Γ ∣ Δ ⊨ k₁ ~ k₂ ∶ B₁ ⇒ B₂) (hn : Γ ∣ ⬝ ⊨ n₁ ~ n₂ ∶ B₁) : Γ ∣ Δ ⊨ (k₁[n₁]) ~ (k₂[n₂]) ∶ B₂ := by
   intro σ τ hστ js₁ js₂ hjs; rw [substPlug, substPlug]
   exact hk hστ hjs (hn hστ .nil)
 
-theorem semPlug {Γ Δ n₁ n₂ k B₁ B₂} (hk : Γ ∣ Δ ⊢ k ∶ B₁ ⇒ B₂) (hn : Γ ∣ ⬝ ⊨ n₁ ~ n₂ ∶ B₁) : Γ ∣ Δ ⊨ (k [ n₁ ]) ~ (k [ n₂ ]) ∶ B₂ :=
+theorem semPlug {Γ δ} {Δ : Dtxt δ} {n₁ n₂ k B₁ B₂} (hk : Γ ∣ Δ ⊢ k ∶ B₁ ⇒ B₂) (hn : Γ ∣ ⬝ ⊨ n₁ ~ n₂ ∶ B₁) : Γ ∣ Δ ⊨ (k [ n₁ ]) ~ (k [ n₂ ]) ∶ B₂ :=
   semK.plug (soundK hk) hn
 
 /-*--------------------------------------
   Plugging commutes with configurations
 --------------------------------------*-/
 
-theorem semKletin {Γ Δ n m k B₁ B₂} (hk : Γ ∣ Δ ⊢ k ∶ B₁ ⇒ B₂) (h : Γ ∣ ⬝ ⊢ letin n m ∶ B₁) :
+theorem semKletin {Γ δ} {Δ : Dtxt δ} {n m k B₁ B₂} (hk : Γ ∣ Δ ⊢ k ∶ B₁ ⇒ B₂) (h : Γ ∣ ⬝ ⊢ letin n m ∶ B₁) :
   Γ ∣ Δ ⊨ (k [letin n m]) ~ letin n ((renameK succ k) [m]) ∶ B₂ := by
   induction hk generalizing n m
-  case nil => exact soundCom h
+  case nil => exact soundCom (wtRenameJ (λ _ _ _ mem ↦ by cases mem) h)
   case app hv hk ih => exact semCom.trans (semPlug hk (appLet h hv)) (ih (wtLetApp h hv))
   case letin hm => exact letLet h hm
   case fst hk ih => exact semCom.trans (semPlug hk (fstLet h)) (ih (wtLetFst h))
   case snd hk ih => exact semCom.trans (semPlug hk (sndLet h)) (ih (wtLetSnd h))
 
-theorem semKcase {Γ Δ v m₁ m₂ k B₁ B₂} (hk : Γ ∣ Δ ⊢ k ∶ B₁ ⇒ B₂) (h : Γ ∣ ⬝ ⊢ case v m₁ m₂ ∶ B₁) :
+theorem semKcase {Γ δ} {Δ : Dtxt δ} {v m₁ m₂ k B₁ B₂} (hk : Γ ∣ Δ ⊢ k ∶ B₁ ⇒ B₂) (h : Γ ∣ ⬝ ⊢ case v m₁ m₂ ∶ B₁) :
   Γ ∣ Δ ⊨ (k [case v m₁ m₂]) ~ case v ((renameK succ k) [m₁]) ((renameK succ k) [m₂]) ∶ B₂ := by
   induction hk generalizing v m₁ m₂
-  case nil => exact soundCom h
+  case nil => exact soundCom (wtRenameJ (λ _ _ _ mem ↦ by cases mem) h)
   case app hv hk ih => exact semCom.trans (semPlug hk (appCase h hv)) (ih (wtCaseApp h hv))
   case letin hm => exact letCase h hm
   case fst hk ih => exact semCom.trans (semPlug hk (fstCase h)) (ih (wtCaseFst h))
@@ -519,9 +541,9 @@ theorem semKcase {Γ Δ v m₁ m₂ k B₁ B₂} (hk : Γ ∣ Δ ⊢ k ∶ B₁ 
   Jumpification preserves semantic equivalence
 ---------------------------------------------*-/
 
-theorem semJumpPlug {Γ Δ k k' m n B₁ B₂} (hk : Γ ∣ Δ ⊢ k ∶ B₁ ⇒ B₂) (hn : Γ ∣ ⬝ ⊢ n ∶ B₁) (e : k.jumpify = .yes k' m) :
+theorem semJumpPlug {Γ δ} {Δ : Dtxt δ} {k k' m n B₁ B₂} (hk : Γ ∣ Δ ⊢ k ∶ B₁ ⇒ B₂) (hn : Γ ∣ ⬝ ⊢ n ∶ B₁) (e : k.jumpify = .yes k' m) :
   Γ ∣ Δ ⊨ (k [ n ]) ~ join m (k' [ n ]) ∶ B₂ := by
-  induction hk generalizing k' n
+  induction hk generalizing n
   case nil => cases e
   case letin hm =>
     simp at e; let ⟨ek, em⟩ := e; subst ek em
@@ -536,57 +558,45 @@ theorem semJumpPlug {Γ Δ k k' m n B₁ B₂} (hk : Γ ∣ Δ ⊢ k ∶ B₁ �
     rename _ = _ => e
     refine ih ?_ e; constructor <;> assumption
 
--- Should this go in Commutation once it's proven?
-theorem joinJoin {Γ Δ n₁ n₂ m A B} (hn₁ : Γ ∷ A ∣ Δ ⊢ n₁ ∶ B) (hn₂ : Γ ∷ A ∣ Δ ⊢ n₂ ∶ B) (hm : Γ ∣ Δ ∷ A ↗ B ⊢ m ∶ B) :
-  Γ ∣ Δ ⊨ join (join (renameCom (lift succ) n₁) n₂) m ~ join n₁ (join n₂ (renameJCom (lift succ) m)) ∶ B := by
-  intro σ τ hστ js₁ js₂ hjs
-  refine ℰ.bwdsRejoin .refl .refl ?_
-  have hjsn₁ := semDtxt.cons hjs (λ hvw ↦
-    have hn := soundCom hn₁ (semCtxt.cons hvw hστ) hjs
-    by rw [← substUnion σ, ← substUnion τ] at hn; exact hn)
-  have what := soundCom hm hστ hjsn₁; simp at what
-  sorry
-
-theorem semJumpA {Γ Δ k k' m m' B₁ B₂} (mj : m.joinless) (hk : Γ ∣ Δ ⊢ k ∶ B₁ ⇒ B₂) (hm : Γ ∣ ⬝ ⊢ m ∶ B₁) (e : k.jumpify = .yes k' m') :
-  Γ ∣ Δ ⊨ ⟦m⟧ₘ k ~ join m' (⟦m⟧ₘ k') ∶ B₂ := by
-  generalize eΔ : Dtxt.nil = Δ' at hm
-  mutual_induction hm generalizing k k' m' mj eΔ
-  all_goals subst eΔ; intro σ τ
+theorem semJumpA {Γ δ δ'} {Δ : Dtxt δ} {Δ' : Dtxt δ'} {k k' m m' B₁ B₂} (le : δ' ≤ δ) (mj : m.joinless) (hk : Γ ∣ Δ ⊢ k ∶ B₁ ⇒ B₂) (hm : Γ ∣ Δ' ⊢ m ∶ B₁) (e : k.jumpify = .yes k' m') :
+  Γ ∣ Δ ⊨ ⟦m⟧ₘ k # le ~ join m' (⟦m⟧ₘ k' # .step le) ∶ B₂ := by
+  mutual_induction hm generalizing δ Δ k k' m' mj
+  all_goals intro σ τ
   -- impossible
   case join | jump => cases mj
   -- plugging cases
   case force hv => exact semJumpPlug hk (.force (.preservation mj hv)) e
-  case lam hm _ => simp at mj; exact semJumpPlug hk (.lam (.preservation mj .nil hm)) e
+  case lam hm _ => simp at mj; exact semJumpPlug hk (.lam (.preservation .refl mj .nil hm)) e
   case ret hv => exact semJumpPlug hk (.ret (.preservation mj hv)) e
   case prod hm₁ hm₂ _ _ =>
-    simp at mj; let ⟨mj₁, mj₂⟩ := mj
-    exact semJumpPlug hk (.prod (.preservation mj₁ .nil hm₁) (.preservation mj₂ .nil hm₂)) e
+    let ⟨mj₁, mj₂⟩ := mj
+    exact semJumpPlug hk (.prod (.preservation _ mj₁ .nil hm₁) (.preservation _ mj₂ .nil hm₂)) e
   -- extended continuation cases
   case app v _ _ _ hv ih =>
     let ⟨mj, vj⟩ := mj
-    have goal := ih (k' := .app ⟦v⟧ᵥ k') (m' := m') mj (.app (.preservation vj hv) hk)
-    simp only [K.jumpify, e] at goal; exact goal ⟨⟩ ⟨⟩
+    have goal := ih (k' := .app ⟦v⟧ᵥ k') (m' := m') (zero_le δ) mj (.app (.preservation vj hv) hk)
+    simp only [K.jumpify, e] at goal; exact goal ⟨⟩
   case fst ih =>
-    have goal := ih (k' := .fst k') (m' := m') mj (.fst hk)
-    simp only [K.jumpify, e] at goal; exact goal ⟨⟩ ⟨⟩
+    have goal := ih (k' := .fst k') (m' := m') (zero_le δ) mj (.fst hk)
+    simp only [K.jumpify, e] at goal; exact goal ⟨⟩
   case snd ih =>
-    have goal := ih (k' := .snd k') (m' := m') mj (.snd hk)
-    simp only [K.jumpify, e] at goal; exact goal ⟨⟩ ⟨⟩
+    have goal := ih (k' := .snd k') (m' := m') (zero_le δ) mj (.snd hk)
+    simp only [K.jumpify, e] at goal; exact goal ⟨⟩
   -- configuration cases
-  case letin Γ n m A B hn ihn hm ihm =>
+  case letin Γ _ n m A B hn hm ihn ihm =>
     intro hστ js₁ js₂ hjs; simp
     let ⟨nj, mj⟩ := mj
-    have ahm := ComWt.preservation mj hk.weaken hm
-    have ahn := ComWt.preservation (Δ := Δ ∷ A ↗ B₂) nj (.letin (.jump .here (.var .here))) hn
-    have aihm : Γ ∷ A ∣ Δ ⊨ (⟦ m ⟧ₘ renameK succ k) ~ join (renameCom (lift succ) m') (⟦ m ⟧ₘ renameK succ k') ∶ B₂ :=
-      λ {σ τ} ↦ ihm mj hk.weaken (Jump.rename e) rfl (σ := σ) (τ := τ)
+    have ⟨A', hk', hm'⟩ := wtK.jumpify hk e
+    have ahm := ComWt.preservation le mj hk.weaken hm
+    have ahn := ComWt.preservation (Δ := Δ ∷ A ↗ B₂) (zero_le (δ + 1)) nj (.letin (.jump .here (.var .here))) hn
+    have aihm : Γ ∷ A ∣ Δ ⊨ (⟦ m ⟧ₘ renameK succ k # le) ~ join (renameCom (lift succ) m') (⟦ m ⟧ₘ renameK succ k' # .step le) ∶ B₂ :=
+      λ {σ τ} ↦ ihm le mj hk.weaken (Jump.rename e) (σ := σ) (τ := τ)
     have hττ : Γ ⊨ τ ~ τ := semCtxt.trans hστ.sym hστ
     have hjs₂₂ : Δ ⊨ js₂ ~ js₂ := semDtxt.trans hjs.sym hjs
-    apply ℰ.trans (ihn nj (wtK.letin ahm) rfl rfl hστ hjs)
+    apply ℰ.trans (ihn (zero_le δ) nj (wtK.letin ahm) rfl hστ hjs)
     apply ℰ.trans (semCom.join aihm (soundCom ahn) hττ hjs₂₂)
-    apply ℰ.trans (joinJoin ?_ ?_ ?_ hττ hjs₂₂); simp
+    apply ℰ.trans (joinJoin ?_ ?_ ahn hττ hjs₂₂); simp
     rw [← rejoin.eq_2 _ (m'⦃⇑ τ⦄), ← rejoin.eq_2 _ (m'⦃⇑ τ⦄)]
-    apply ℰ.bwdsRejoin .refl .refl ?_
     all_goals sorry
   case case => sorry
 
@@ -596,9 +606,9 @@ theorem semJumpA {Γ Δ k k' m m' B₁ B₂} (mj : m.joinless) (hk : Γ ∣ Δ �
 
 theorem soundA {Γ} :
   (∀ {v} {A : ValType}, v.joinless → Γ ⊢ v ∶ A → Γ ⊨ v ~ ⟦v⟧ᵥ ∶ A) ∧
-  (∀ {Δ m k₁ k₂} {B₁ B₂ : ComType}, m.joinless →
+  (∀ {δ} {Δ : Dtxt δ} {m k₁ k₂} {B₁ B₂ : ComType}, m.joinless →
     Γ ∣ ⬝ ⊢ m ∶ B₁ → Γ ∣ Δ ⊢ k₁ ∶ B₁ ⇒ B₂ → Γ ∣ Δ ⊢ k₂ ∶ B₁ ⇒ B₂ →
-    Γ ∣ Δ ⊨ k₁ ~ k₂ ∶ B₁ ⇒ B₂ → Γ ∣ Δ ⊨ (k₁[m]) ~ ⟦m⟧ₘ k₂ ∶ B₂) := by
+    Γ ∣ Δ ⊨ k₁ ~ k₂ ∶ B₁ ⇒ B₂ → Γ ∣ Δ ⊨ (k₁[m]) ~ ⟦m⟧ₘ k₂ # zero_le δ ∶ B₂) := by
   refine ⟨λ vj h ↦ ?val, λ mj h wtk₁ wtk₂ hk ↦ ?com⟩
   case' com => generalize e : Dtxt.nil = Δ' at h
   mutual_induction h, h
@@ -676,8 +686,10 @@ theorem soundA {Γ} :
   case inr ih => exact 𝒱.inr (ih vj hστ)
   case thunk ih => exact 𝒱.thunk (ih vj .nil .nil (soundK .nil) rfl hστ .nil)
 
-theorem soundAnil {Γ m B} (mj : m.joinless) (h : Γ ∣ ⬝ ⊢ m ∶ B) : Γ ∣ ⬝ ⊨ m ~ ⟦m⟧ₘ ∶ B :=
-  soundA.right mj h .nil .nil semK.nil
+theorem soundAnil {Γ m B} (mj : m.joinless) (h : Γ ∣ ⬝ ⊢ m ∶ B) : Γ ∣ ⬝ ⊨ m ~ ⟦m⟧ₘ ∶ B := by
+  intro σ τ hστ js₁ js₂ hjs
+  have goal := soundA.right mj h .nil .nil semK.nil hστ hjs
+  simp at goal; rw [weakenJCom0] at goal; exact goal
 
 /-*------------------------------------------------------------
   A-normalized ground returners compute the same normal forms
@@ -712,5 +724,5 @@ theorem retGroundA {m n A} (mj : m.joinless) (h : ⬝ ∣ ⬝ ⊢ m ∶ F A) (g 
   simp [nfm.steps rn, ra']
 
 theorem retGroundACK {m n A} (mj : m.joinless) (h : ⬝ ∣ ⬝ ⊢ m ∶ F A) (g : isGround A) (nm : nf n) :
-  ⟨m, []⟩ ⤳⋆ ⟨n, []⟩ → ⟨⟦m⟧ₘ, []⟩ ⤳⋆ ⟨n, []⟩ :=
+  ⟨0, m, .nil⟩ ⤳⋆ ⟨0, n, .nil⟩ → ⟨0, ⟦m⟧ₘ, .nil⟩ ⤳⋆ ⟨0, n, .nil⟩ :=
   λ r ↦ evalStep nm (retGroundA mj h g ⟨stepEvalsNil r, nm⟩)
